In progress refactoring into a separate bintree module

Veritas.Merkle.fsti
@@ -3,25 +3,6 @@ module Veritas.Merkle
 open FStar.BitVector
 open Veritas.Memory
 
-(* Nodes in an infinite binary tree *)
-type bin_tree_node = 
-  | Root: bin_tree_node 
-  | LeftChild: n:bin_tree_node -> bin_tree_node
-  | RightChild: n:bin_tree_node -> bin_tree_node
-
-(* Depth of a binary tree node *)
-let rec depth (n:bin_tree_node): Tot nat = 
-  match n with 
-  | Root -> 0
-  | LeftChild n' -> 1 + depth n'
-  | RightChild n' -> 1 + depth n'
-
-(* Parent of a node *)
-let parent (n:bin_tree_node{~(Root? n)}): Tot bin_tree_node = 
-  match n with
-  | LeftChild n' -> n'
-  | RightChild n' -> n'
-
 (* Merkle address is simply a bin_tree_node of bounded depth *)
 type merkle_addr = n:bin_tree_node{depth n <= addr_size}
 
@@ -107,61 +88,6 @@ let rec merklefn (a:merkle_addr) (mem: memory): Tot (merkle_payload_of_addr a)
   then MkLeaf (mem (merkle_leaf_to_addr a))
   else MkInternal (hashfn (merklefn (LeftChild a) mem))
                   (hashfn (merklefn (RightChild a) mem))
-
-(* Is d descendant of a *)
-val is_desc (d a: bin_tree_node): Tot bool
-
-(* Every node is a descendant of root *)
-val lemma_root_is_univ_ancestor (a: bin_tree_node):
-  Lemma (is_desc a Root)
-
-(* Every node is a descendant of itself *)
-val lemma_desc_reflexive (a: bin_tree_node):
-  Lemma (is_desc a a)
-
-(* descendant is a transitive relation *)
-val lemma_desc_transitive (a b c: bin_tree_node):
-  Lemma (is_desc a b /\ is_desc b c ==> is_desc a c)
-
-(* descendant depth >= ancestor depth *)
-val lemma_desc_depth_monotonic (d a: bin_tree_node):
-  Lemma (requires (is_desc d a))
-        (ensures (depth d >= depth a))
-
-(* proper descendant *)
-let is_proper_desc (d a: bin_tree_node) = is_desc d a && d <> a
-
-(* Each node is a descendant of its parent *)
-val lemma_parent_ancestor (a: bin_tree_node{~(Root? a)}):
-  Lemma (is_proper_desc a (parent a))
-
-(* parent is a descendant of a proper ancestor *)
-val lemma_parent_desc_of_proper_ancestor (d:bin_tree_node{~(Root? d)}) (a:bin_tree_node {is_proper_desc d a}):
-  Lemma (is_desc (parent d) a)
-
-(* proper descendant depth > ancestor depth *)
-val lemma_proper_desc_depth_monotonic (d a: bin_tree_node):
-  Lemma (requires (is_proper_desc d a))
-        (ensures (depth d > depth a))
-
-(* Two ancestors of a node are ancestor/descendant of one another *)
-val lemma_two_ancestors_related (d: bin_tree_node) (a1 a2: bin_tree_node):
-  Lemma (requires (is_desc d a1 /\ is_desc d a2))
-        (ensures (is_desc a1 a2 \/ is_desc a2 a1))
-
-(* descendant is a transitive relation *)
-val lemma_proper_desc_transitive1 (a b c: bin_tree_node):
-  Lemma (is_proper_desc a b /\ is_desc b c ==> is_proper_desc a c)
-
-(* descendant is a transitive relation *)
-val lemma_proper_desc_transitive2 (a b c: bin_tree_node):
-  Lemma (is_desc a b /\ is_proper_desc b c ==> is_proper_desc a c)
-
-(* a proper descendant is a descendant of either left or right child *)
-val lemma_proper_desc_left_or_right (d: bin_tree_node) (a: bin_tree_node {is_proper_desc d a}):
-  Lemma (is_desc d (LeftChild a) /\ ~ (is_desc d (RightChild a)) \/
-         is_desc d (RightChild a) /\ ~ (is_desc d (LeftChild a)))
-        [SMTPat (is_proper_desc d a)]
         
 type desc_hash = 
   | Empty: desc_hash
