Veritas.BinTree.fsti
@@ -1,0 +1,99 @@
+module Veritas.BinTree
+
+(* Nodes in an infinite binary tree *)
+type bin_tree_node = 
+  | Root: bin_tree_node 
+  | LeftChild: n:bin_tree_node -> bin_tree_node
+  | RightChild: n:bin_tree_node -> bin_tree_node
+
+(* non-root binary tree node *)
+type non_root_node = (n:bin_tree_node{~(Root? n)})
+
+(* Depth of a binary tree node *)
+let rec depth (n:bin_tree_node): Tot nat = 
+  match n with 
+  | Root -> 0
+  | LeftChild n' -> 1 + depth n'
+  | RightChild n' -> 1 + depth n'
+
+(* Parent of a node *)
+let parent (n:non_root_node): Tot bin_tree_node = 
+  match n with
+  | LeftChild n' -> n'
+  | RightChild n' -> n'
+
+(* Possible child node direction *)
+type bin_tree_dir = 
+  | Left
+  | Right
+
+(* Child node with a specified direction (left|right) *)
+let child (d:bin_tree_dir) (n:bin_tree_node) = 
+  match d with
+  | Left -> LeftChild n
+  | Right -> RightChild n
+
+(* Is d descendant of a *)
+val is_desc (d a: bin_tree_node): Tot bool
+
+(* in an ancestor-desc relationship *)
+let is_anc_desc_sym (a1 a2: bin_tree_node): bool = 
+  is_desc a1 a2 || is_desc a2 a1
+
+(* unrelated in terms of ancestor-desc *)
+let non_anc_desc (a1 a2: bin_tree_node): bool = 
+  not (is_anc_desc_sym a1 a2)
+
+(* Every node is a descendant of root *)
+val lemma_root_is_univ_ancestor (a: bin_tree_node):
+  Lemma (is_desc a Root)
+
+(* Every node is a descendant of itself *)
+val lemma_desc_reflexive (a: bin_tree_node):
+  Lemma (is_desc a a)
+
+(* descendant is a transitive relation *)
+val lemma_desc_transitive (a b c: bin_tree_node):
+  Lemma (is_desc a b /\ is_desc b c ==> is_desc a c)
+
+(* descendant depth >= ancestor depth *)
+val lemma_desc_depth_monotonic (d a: bin_tree_node):
+  Lemma (requires (is_desc d a))
+        (ensures (depth d >= depth a))
+
+(* proper descendant *)
+let is_proper_desc (d a: bin_tree_node) = is_desc d a && d <> a
+
+(* Each node is a descendant of its parent *)
+val lemma_parent_ancestor (a:non_root_node):
+  Lemma (is_proper_desc a (parent a))
+
+(* parent is a descendant of a proper ancestor *)
+val lemma_parent_desc_of_proper_ancestor (d:non_root_node) (a:bin_tree_node {is_proper_desc d a}):
+  Lemma (is_desc (parent d) a)
+
+(* proper descendant depth > ancestor depth *)
+val lemma_proper_desc_depth_monotonic (d a: bin_tree_node):
+  Lemma (requires (is_proper_desc d a))
+        (ensures (depth d > depth a))
+
+(* Two ancestors of a node are ancestor/descendant of one another *)
+val lemma_two_ancestors_related (d: bin_tree_node) (a1 a2: bin_tree_node):
+  Lemma (requires (is_desc d a1 /\ is_desc d a2))
+        (ensures (is_anc_desc_sym a1 a2))
+
+(* descendant is a transitive relation *)
+val lemma_proper_desc_transitive1 (a b c: bin_tree_node):
+  Lemma (is_proper_desc a b /\ is_desc b c ==> is_proper_desc a c)
+
+(* descendant is a transitive relation *)
+val lemma_proper_desc_transitive2 (a b c: bin_tree_node):
+  Lemma (is_desc a b /\ is_proper_desc b c ==> is_proper_desc a c)
+
+val lemma_siblings_non_anc_desc (n:bin_tree_node):
+  Lemma (non_anc_desc (LeftChild n) (RightChild n))
+
+(* a proper descendant is a descendant of either left or right child *)
+val lemma_proper_desc_left_or_right (d: bin_tree_node) (a: bin_tree_node {is_proper_desc d a}):
+  Lemma (is_desc d (LeftChild a) /\ ~ (is_desc d (RightChild a)) \/
+         is_desc d (RightChild a) /\ ~ (is_desc d (LeftChild a)))
